

Bonusaufgabe 3

Sei $B = \{b_1, b_2, b_3, b_4\}$ eine Basis des \mathbb{R}^4 und sei $a = 3b_1 - 4b_2 + 5b_3 - 2b_4 \in \mathbb{R}^4$.

z.z. $B' = \{a, b_2, b_3, b_4\}$ l.u. ist.

$$\lambda_1 a + \lambda_2 b_2 + \lambda_3 b_3 + \lambda_4 b_4 = 0$$

da $a \in L(B)$, existieren Koeffizienten $3, -4, 5, -2 \in \mathbb{R}^4$, sodass

$$a = 3b_1 - 4b_2 + 5b_3 - 2b_4 \quad \text{d.h.}$$

$$\lambda_1 \cdot (3b_1 - 4b_2 + 5b_3 - 2b_4) + \lambda_2 b_2 + \lambda_3 b_3 + \lambda_4 b_4 = 0$$

$$3\lambda_1 b_1 + (-4\lambda_1 + \lambda_2) b_2 + (5\lambda_1 + \lambda_3) b_3 + (-2\lambda_1 + \lambda_4) b_4 = 0$$

$$3\lambda_1 = 0 \implies \lambda_1 = 0$$

$$-4\lambda_1 + \lambda_2 = 0 \implies \lambda_2 = 0$$

$$5\lambda_1 + \lambda_3 = 0 \implies \lambda_3 = 0$$

$$-2\lambda_1 + \lambda_4 = 0 \implies \lambda_4 = 0$$

Damit sind alle Koeffizienten Null und B' l.u.

qed